Prove progress and preservation for the STLC

STLC.thy
@@ -1,12 +1,11 @@
 theory STLC
-  imports "thys/MRBNF_Recursor"
+  imports "thys/MRBNF_Recursor" "HOL-Library.FSet"
 begin
 
 (* TODO: Move into MRBNF_Recursor.thy *)
 ML_file \<open>./Tools/mrbnf_recursor_tactics.ML\<close>
 ML_file \<open>./Tools/mrbnf_recursor.ML\<close>
 
-ML_file \<open>./Tools/mrbnf_vvsubst_tactics.ML\<close>
 ML_file \<open>./Tools/mrbnf_vvsubst.ML\<close>
 
 datatype \<tau> = Unit | Arrow \<tau> \<tau> (infixr "\<rightarrow>" 40)
@@ -265,64 +264,86 @@ lemma Abs_avoid: "|A::'a::var_terms_pre set| <o |UNIV::'a set| \<Longrightarrow>
   apply assumption
   done
 
+lemma TT_fresh_induct_param:
+  fixes x::"'a::var_terms_pre terms" and K::"'b \<Rightarrow> 'a set"
+  assumes "\<forall>\<rho>. |K \<rho>| <o |UNIV::'a set|"
+and Var: "\<And>a \<rho>. P (Var a) \<rho>"
+and App: "\<And>e1 e2 \<rho>. \<lbrakk> \<forall>\<rho>. P e1 \<rho> ; \<forall>\<rho>. P e2 \<rho> \<rbrakk> \<Longrightarrow> P (App e1 e2) \<rho>"
+and Abs: "\<And>x \<tau> e \<rho>. \<lbrakk> x \<notin> K \<rho> ; \<forall>\<rho>. P e \<rho> \<rbrakk> \<Longrightarrow> P (Abs x \<tau> e) \<rho>"
+shows "\<forall>\<rho>. P x \<rho>"
+  apply (rule allI)
+  subgoal for \<rho>
+  apply (rule spec[OF terms.TT_fresh_co_induct_param[of "UNIV::'b set", unfolded ball_UNIV, of K]])
+   apply (rule spec[OF assms(1)])
+  subgoal premises IHs for v \<rho>
+    apply (rule Abs_terms_pre_cases[of v])
+    subgoal for y
+      apply (rule sum.exhaust[of y])
+       apply hypsubst
+      apply (rule Var[unfolded Var_def])
+      subgoal for y2
+        apply (rule sum.exhaust[of y2])
+        subgoal for y3
+          apply (rule prod.exhaust[of y3])
+          apply hypsubst
+          apply (frule arg_cong[of _ _ "Abs_terms_pre"])
+        apply (rotate_tac -1)
+          apply (drule arg_cong[of _ _ terms_ctor])
+          unfolding App_def[symmetric]
+          apply (drule App_set4)
+          apply (erule conjE)
+          apply (rule App)
+           apply (rule allI)
+           apply (rule IHs(2))
+            apply hypsubst
+            apply assumption
+           apply (rule UNIV_I)
+          apply (rule allI)
+          apply (rule IHs(2))
+           apply hypsubst
+           apply assumption
+          apply (rule UNIV_I)
+          done
+        subgoal for y3
+          apply (rule prod.exhaust[of y3])
+          apply hypsubst
+          subgoal for x y4
+            apply (rule prod.exhaust[of y4])
+            apply hypsubst
+            apply (frule arg_cong[of _ _ terms_ctor])
+            unfolding Abs_def[symmetric]
+            apply (frule Abs_set3)
+            apply (erule exE conjE)+
+            apply (rule iffD2[OF arg_cong2[OF _ refl, of _ _ P]])
+            apply (rule trans)
+             apply (rule sym)
+              apply assumption
+             apply (rotate_tac -3)
+             apply assumption
+            apply (rule Abs)
+             apply (rule IHs)
+             apply assumption
+            apply (rule allI)
+            apply (rule IHs(1))
+             apply assumption
+            apply (rule UNIV_I)
+            done
+          done
+        done
+      done
+    done
+  done
+  done
+
 lemma TT_fresh_induct[case_names Bound Var App Abs]:
   assumes bound: "|A::'a set| <o |UNIV::'a::var_terms_pre set|"
   and Var: "\<And>a. P (Var a)"
   and App: "\<And>e1 e2. P e1 \<Longrightarrow> P e2 \<Longrightarrow> P (App e1 e2)"
   and Abs: "\<And>x \<tau> e. x \<notin> A \<Longrightarrow> P e \<Longrightarrow> P (Abs x \<tau> e)"
 shows "P x"
-  apply (rule terms.TT_fresh_co_induct)
-   apply (rule bound)
-  subgoal for v
-    apply (rule Abs_terms_pre_cases[of v])
-    subgoal for y
-    apply (rule sum.exhaust[of y])
-     apply (raw_tactic \<open>hyp_subst_tac @{context} 1\<close>)
-    unfolding Var_def[symmetric]
-     apply (rule Var)
-    subgoal for y2
-      apply (rule sum.exhaust[of y2])
-       apply (raw_tactic \<open>hyp_subst_tac @{context} 1\<close>)
-      subgoal for y3
-        apply (rule prod.exhaust[of y3])
-        apply (raw_tactic \<open>hyp_subst_tac @{context} 1\<close>)
-        apply (frule arg_cong[of _ _ "Abs_terms_pre"])
-        apply (rotate_tac -1)
-        apply (drule arg_cong[of _ _ terms_ctor])
-        unfolding App_def[symmetric]
-        apply (drule App_set4)
-        apply (erule conjE)
-        apply (rule App)
-         apply (raw_tactic \<open>hyp_subst_tac @{context} 1\<close>)
-         apply assumption
-        apply (raw_tactic \<open>hyp_subst_tac @{context} 1\<close>)
-        apply assumption
-        done
-      subgoal for y3
-        apply (rule prod.exhaust[of y3])
-        subgoal for x b
-          apply (rule prod.exhaust[of b])
-          apply (frule arg_cong[of _ _ terms_ctor])
-          apply (rotate_tac -1)
-          apply (drule sym[THEN trans[rotated]])
-           defer
-           apply (rotate_tac -1)
-           apply (drule sym)
-           apply (drule Abs_set3)
-           apply (erule exE conjE)+
-           apply (rule iffD2[OF arg_cong[of _ _ P]])
-          apply assumption
-           apply (rule Abs)
-            apply assumption
-           apply assumption
-          apply (raw_tactic \<open>hyp_subst_tac @{context} 1\<close>)
-          unfolding Abs_def[symmetric]
-          apply (rule refl)
-          done
-        done
-      done
-    done
-  done
+  apply (rule spec[OF TT_fresh_induct_param[of _ "\<lambda>x \<rho>. P x"]])
+     apply (rule allI)
+     apply (rule assms | assumption | erule allE)+
   done
 
 lemmas TT_plain_induct = TT_fresh_induct[OF emp_bound, case_names Var App Abs]
@@ -349,6 +370,7 @@ lemma bij_not_eq_twice: "bij g \<Longrightarrow> g a \<noteq> a \<Longrightarrow
   by simp
 lemma bij_not_equal_iff: "bij f \<Longrightarrow> a \<noteq> b \<longleftrightarrow> f a \<noteq> f b"
   by simp
+lemma not_fun_cong: "f a \<noteq> f b \<Longrightarrow> a \<noteq> b" by blast
 lemma fst_o_f: "fst \<circ> (\<lambda>(x, y). (f x, g x y)) = f \<circ> fst"
   by auto
 lemma id_o_commute: "id \<circ> f = f \<circ> id" by simp
@@ -401,17 +423,15 @@ lemma rrename_VVr:
   shows "rrename_terms f (VVr a) = VVr (f a)"
   unfolding VVr_def terms.rrename_cctors[OF assms]
   apply (rule arg_cong[of _ _ terms_ctor])
-  apply (rule trans)
-   apply (rule fun_cong[OF \<eta>_natural[unfolded comp_def]])
-     apply (rule assms)+
-  apply (rule refl)
+  apply (rule fun_cong[OF \<eta>_natural[unfolded comp_def]])
+    apply (rule assms)+
   done
 
 definition SSupp :: "('a::var_terms_pre \<Rightarrow> 'a terms) \<Rightarrow> 'a set" where
   "SSupp f \<equiv> { a. f a \<noteq> VVr a }"
 
 definition IImsupp :: "('a::var_terms_pre \<Rightarrow> 'a terms) \<Rightarrow> 'a set" where
-  "IImsupp f \<equiv> SSupp f \<union> (\<Union> a \<in> SSupp f. FFVars_terms (f a))"
+  "IImsupp f \<equiv> SSupp f \<union> (\<Union>a\<in>SSupp f. FFVars_terms (f a))"
 
 lemma in_IImsupp: "f a \<noteq> VVr a \<Longrightarrow> z \<in> FFVars_terms (f a) \<Longrightarrow> z \<in> IImsupp f"
   unfolding IImsupp_def SSupp_def
@@ -496,11 +516,8 @@ lemma SSupp_VVr_empty: "SSupp VVr = {}"
   unfolding SSupp_def
   apply (rule iffD2[OF set_eq_iff])
   apply (rule allI)
-  apply (rule iffI)
-   apply (drule iffD1[OF mem_Collect_eq])
-  unfolding atomize_not not_not empty_iff
-   apply (rule refl)
-  apply (erule FalseE)
+  unfolding mem_Collect_eq HOL.simp_thms(6) empty_iff
+  apply (rule not_True_eq_False)
   done
 
 lemma IImsupp_VVr_empty: "IImsupp VVr = {}"
@@ -517,8 +534,20 @@ lemma SSupp_comp_subset:
   fixes f::"'a::var_terms_pre \<Rightarrow> 'a terms" and g::"'a \<Rightarrow> 'a"
   assumes "|supp g| <o |UNIV::'a set|" "bij g"
   shows "SSupp (f \<circ> g) \<subseteq> SSupp f \<union> supp g"
-  unfolding SSupp_def supp_def
-  by auto
+  unfolding SSupp_def supp_def subset_iff mem_Collect_eq Un_iff comp_def
+  apply (rule allI)
+  apply (rule impI)
+  subgoal for t
+    apply (rule case_split[of "g t = t"])
+     apply (drule iffD1[OF arg_cong2[OF _ refl, of _ _ "(\<noteq>)"], rotated])
+      apply (rule arg_cong[of _ _ f])
+      apply assumption
+     apply (rule disjI1)
+     apply assumption
+    apply (rule disjI2)
+    apply assumption
+    done
+  done
 
 lemma SSupp_comp_bound:
   fixes f::"'a::var_terms_pre \<Rightarrow> 'a terms" and g::"'a \<Rightarrow> 'a"
@@ -530,10 +559,24 @@ lemma SSupp_comp_bound:
 
 lemma SSupp_comp_rename_subset:
   fixes f::"'a::var_terms_pre \<Rightarrow> 'a terms" and g::"'a \<Rightarrow> 'a"
-  assumes "|supp g| <o |UNIV::'a set|" "bij g"
+  assumes "bij g" "|supp g| <o |UNIV::'a set|"
   shows "SSupp (rrename_terms g \<circ> f) \<subseteq> SSupp f \<union> supp g"
   unfolding SSupp_def supp_def
-  by (auto simp: rrename_VVr assms)
+  apply (rule subsetI)
+  unfolding mem_Collect_eq Un_iff comp_def
+  subgoal for x
+    apply (rule case_split[of "f x = VVr x"])
+     apply (drule iffD1[OF arg_cong2[OF _ refl, of _ _ "(\<noteq>)"], rotated])
+      apply (rule arg_cong[of _ _ "rrename_terms g"])
+      apply assumption
+    unfolding rrename_VVr[OF assms]
+     apply (rule disjI2)
+     apply (rule not_fun_cong)
+     apply assumption
+    apply (rule disjI1)
+    apply assumption
+    done
+  done
 
 lemma SSupp_comp_rename_bound:
   fixes f::"'a::var_terms_pre \<Rightarrow> 'a terms" and g::"'a \<Rightarrow> 'a"
@@ -544,7 +587,10 @@ lemma SSupp_comp_rename_bound:
   done
 
 typedef 'a::var_terms_pre SSfun = "{ f::'a \<Rightarrow> 'a terms. |SSupp f| <o |UNIV::'a set| }"
-  by (auto intro!: exI[of _ VVr] simp: SSupp_VVr_bound)
+  apply (rule exI)
+  apply (rule iffD2[OF mem_Collect_eq])
+  apply (rule SSupp_VVr_bound)
+  done
 
 lemma IImsupp_comp_image:
   assumes "bij f" "|supp (f::'a::var_terms_pre \<Rightarrow> 'a)| <o |UNIV::'a set|"
@@ -888,7 +934,7 @@ let
     },
     axioms = model_axioms
   } : (Proof.context -> tactic) MRBNF_Recursor.model;
-  
+
   val (rec_res, lthy) = MRBNF_Recursor.create_binding_recursor (Binding.prefix_name "tv") model @{binding tvsubst} lthy
   val _ = @{print} rec_res
   val notes =
@@ -1130,12 +1176,12 @@ shows "FFVars_terms (tvsubst f t) \<subseteq> FFVars_terms t \<union> IImsupp f"
   ])
   done
 
-lemma nexists_inject: "\<nexists>a. f x = f (g a) \<Longrightarrow> \<nexists>a. x = g a" by blast
-
 lemma not_isVVr_free: "\<not>isVVr (terms_ctor x) \<Longrightarrow> set1_terms_pre x = {}"
   apply (rule \<eta>_compl_free)
-  unfolding isVVr_def VVr_def image_iff bex_simps
-  apply (rule nexists_inject)
+  unfolding isVVr_def VVr_def image_iff Set.bex_simps not_ex
+  apply (rule allI)
+  apply (erule allE)
+  apply (rule not_fun_cong)
   apply assumption
   done
 
@@ -1145,7 +1191,8 @@ lemma UN_cong: "(\<And>x. x \<in> A \<Longrightarrow> P x = Q x) \<Longrightarro
 lemma IImsupp_Diff: "(\<And>x. x \<in> B \<Longrightarrow> x \<notin> IImsupp f) \<Longrightarrow> (\<Union>a\<in>(A - B). FFVars_terms (f a)) = (\<Union>a\<in>A. FFVars_terms (f a)) - B"
   unfolding atomize_imp
   unfolding atomize_all
-  apply (drule iffD2[OF disjoint_iff])  apply (rule iffD2[OF set_eq_iff])
+  apply (drule iffD2[OF disjoint_iff])
+  apply (rule iffD2[OF set_eq_iff])
   apply (rule allI)
   apply (rule iffI)
    apply (erule UN_E)
@@ -1241,7 +1288,7 @@ lemma FFVars_tvsubst:
        apply (rule iffD2[OF disjoint_iff], rule allI, rule impI)
        apply assumption
       apply (rule iffD2[OF disjoint_iff], rule allI, rule impI)
-    unfolding UN_iff bex_simps
+    unfolding UN_iff Set.bex_simps
       apply (rule ballI)
       apply assumption
      apply assumption
@@ -1283,7 +1330,7 @@ lemma tvsubst_VVr_func: "tvsubst VVr t = t"
         apply (rule conjI)
          apply (rule iffD2[OF disjoint_iff], rule allI, rule impI, assumption)
         apply (rule iffD2[OF disjoint_iff], rule allI, rule impI)
-      unfolding UN_iff bex_simps
+      unfolding UN_iff Set.bex_simps
         apply (rule ballI)
         apply assumption+
       apply (rule arg_cong[of _ _ terms_ctor])
@@ -1314,92 +1361,83 @@ corollary SSupp_upd_VVr_bound: "|SSupp (VVr(a:=(t::'a::var_terms_pre terms)))| <
   apply (rule SSupp_VVr_bound)
   done
 
+lemma supp_subset_id_on: "supp f \<subseteq> A \<Longrightarrow> id_on (B - A) f"
+  unfolding supp_def id_on_def by blast
+
 (* small step semantics *)
 no_notation Set.member  ("(_/ : _)" [51, 51] 50)
-no_notation Set.member  ("(_/ \<in> _)" [51, 51] 50)
 
-fun isin :: "'a * 'b \<Rightarrow> ('a * 'b) list \<Rightarrow> bool" ("(_/ \<in> _)" [51, 51] 50) where
-  "isin _ [] = False"
-| "isin (x, \<tau>) ((y, \<tau>')#ys) = (if x = y then \<tau> = \<tau>' else isin (x, \<tau>) ys)"
+definition fresh :: "'a::var_terms_pre \<Rightarrow> ('a * 'b) fset \<Rightarrow> bool" ("(_/ \<sharp> _)" [51, 51] 50) where
+  "fresh x \<Gamma> \<equiv> x |\<notin>| fst |`| \<Gamma>"
 
-definition fresh :: "'a::var_terms_pre \<Rightarrow> ('a * 'b) list \<Rightarrow> bool" ("(_/ \<sharp> _)" [51, 51] 50) where
-  "fresh x \<Gamma> \<equiv> x \<notin> set (map fst \<Gamma>)"
+lemma isin_rename: "bij f \<Longrightarrow> (f x, \<tau>) |\<in>| map_prod f id |`| \<Gamma> \<longleftrightarrow> (x, \<tau>) |\<in>| \<Gamma>"
+  by force
 
-lemma not_isin_member: "x \<sharp> \<Gamma> \<Longrightarrow> \<not>((x, \<tau>) \<in> \<Gamma>)"
-  by (induction \<Gamma>) (auto simp: fresh_def split!: if_splits)
-lemma isin_member: "(x, \<tau>) \<in> \<Gamma> \<Longrightarrow> Set.member x (set (map fst \<Gamma>))"
-  by (induction \<Gamma>) (auto split!: if_splits)
-lemma isin_rename: "bij f \<Longrightarrow> (f x, \<tau>) \<in> map (map_prod f id) \<Gamma> \<longleftrightarrow> (x, \<tau>) \<in> \<Gamma>"
-  by (induction \<Gamma>) (auto split!: if_splits)
+abbreviation extend :: "('a * \<tau>) fset \<Rightarrow> 'a::var_terms_pre \<Rightarrow> \<tau> \<Rightarrow> ('a * \<tau>) fset" ("(_,_:_)") where
+  "extend \<Gamma> a \<tau> \<equiv> finsert (a, \<tau>) \<Gamma>"
 
 inductive Step :: "'a::var_terms_pre terms \<Rightarrow> 'a terms \<Rightarrow> bool" ("_ \<longrightarrow> _" 25) where
   ST_Beta: "App (Abs x \<tau> e) e2 \<longrightarrow> tvsubst (VVr(x:=e2)) e"
 | ST_App: "e1 \<longrightarrow> e1' \<Longrightarrow> App e1 e2 \<longrightarrow> App e1' e2"
 
-inductive Ty :: "('a::var_terms_pre * \<tau>) list \<Rightarrow> 'a terms \<Rightarrow> \<tau> \<Rightarrow> bool" ("_ \<turnstile>\<^sub>t\<^sub>y _ : _") where
-  Ty_Var: "(x, \<tau>) \<in> \<Gamma> \<Longrightarrow> \<Gamma> \<turnstile>\<^sub>t\<^sub>y Var x : \<tau>"
+inductive Ty :: "('a::var_terms_pre * \<tau>) fset \<Rightarrow> 'a terms \<Rightarrow> \<tau> \<Rightarrow> bool" ("_ \<turnstile>\<^sub>t\<^sub>y _ : _") where
+  Ty_Var: "(x, \<tau>) |\<in>| \<Gamma> \<Longrightarrow> \<Gamma> \<turnstile>\<^sub>t\<^sub>y Var x : \<tau>"
 | Ty_App: "\<lbrakk> \<Gamma> \<turnstile>\<^sub>t\<^sub>y e1 : \<tau>\<^sub>1 \<rightarrow> \<tau>\<^sub>2 ; \<Gamma> \<turnstile>\<^sub>t\<^sub>y e2 : \<tau>\<^sub>1 \<rbrakk> \<Longrightarrow> \<Gamma> \<turnstile>\<^sub>t\<^sub>y App e1 e2 : \<tau>\<^sub>2"
-| Ty_Abs: "\<lbrakk> x \<sharp> \<Gamma> ; (x, \<tau>)#\<Gamma> \<turnstile>\<^sub>t\<^sub>y e : \<tau>\<^sub>2 \<rbrakk> \<Longrightarrow> \<Gamma> \<turnstile>\<^sub>t\<^sub>y Abs x \<tau> e : \<tau> \<rightarrow> \<tau>\<^sub>2"
+| Ty_Abs: "\<lbrakk> x \<sharp> \<Gamma> ; \<Gamma>,x:\<tau> \<turnstile>\<^sub>t\<^sub>y e : \<tau>\<^sub>2 \<rbrakk> \<Longrightarrow> \<Gamma> \<turnstile>\<^sub>t\<^sub>y Abs x \<tau> e : \<tau> \<rightarrow> \<tau>\<^sub>2"
 
-inductive_cases
-  Ty_VarE: "\<Gamma> \<turnstile>\<^sub>t\<^sub>y Var x : \<tau>"
-  and Ty_AppE: "\<Gamma> \<turnstile>\<^sub>t\<^sub>y App e1 e2 : \<tau>\<^sub>2"
-  and Ty_AbsE_aux: "\<Gamma> \<turnstile>\<^sub>t\<^sub>y Abs x \<tau> e : \<tau>'"
+(* Design for better inductive:
 
-print_theorems
+provide additional command `binder_inductive` that takes the name of a normal inductive as argument.
+This uses the map function of the BNFs involved.
+
+binder_inductive Ty where
+  Ty_Abs: x
+
+This opens a proof for all the equalities and implications needed: *)
+
+lemma provided:
+  fixes f::"'a::var_terms_pre \<Rightarrow> 'a"
+  assumes "bij f" "|supp f| <o |UNIV::'a set|"
+  shows
+    (* equivariance *)
+    "(x, \<tau>) |\<in>| \<Gamma> \<Longrightarrow> (f x, \<tau>) |\<in>| map_prod f id |`| \<Gamma>"
+    "x \<sharp> \<Gamma> \<Longrightarrow> f x \<sharp> map_prod f id |`| \<Gamma>"
+    (* equivariance of extend *)
+    "map_prod f id |`| (\<Gamma>,x:\<tau>) = (map_prod f id |`| \<Gamma>),f x:\<tau>"
+    (* freshness *)
+    "\<lbrakk> x \<sharp> \<Gamma> ; \<Gamma>,x:\<tau> \<turnstile>\<^sub>t\<^sub>y e : \<tau>\<^sub>2 \<rbrakk> \<Longrightarrow> x \<notin> \<Union>(Basic_BNFs.fsts ` fset \<Gamma>)"
+   apply (simp add: assms isin_rename)
+  unfolding fresh_def
+  apply (metis Product_Type.fst_comp_map_prod assms(1) bij_not_equal_iff fimageE fset.map_comp)
+   apply simp
+  using fmember_iff_member_fset image_iff apply fastforce
+  done
 
 lemma rename_Ty_aux:
   fixes f::"'a::var_terms_pre \<Rightarrow> 'a"
-  assumes "bij f" "|supp f| <o |UNIV::'a set|" "\<Gamma> \<turnstile>\<^sub>t\<^sub>y e : \<tau>'"
-  shows "map (map_prod f id) \<Gamma> \<turnstile>\<^sub>t\<^sub>y rrename_terms f e : \<tau>'"
+  assumes
+    "bij f" "|supp f| <o |UNIV::'a set|" "\<Gamma> \<turnstile>\<^sub>t\<^sub>y e : \<tau>'"
+  shows "map_prod f id |`| \<Gamma> \<turnstile>\<^sub>t\<^sub>y vvsubst f e : \<tau>'"
   apply (rule Ty.induct[OF assms(3)])
-  unfolding rrename_simps[OF assms(1,2)]
+  unfolding terms_vvsubst_rrename[OF assms(1,2)] rrename_simps[OF assms(1,2)]
     apply (rule Ty_Var)
-  subgoal for x \<tau> \<Gamma>
-    unfolding atomize_imp
-    apply (rule list.induct[of _ \<Gamma>])
-     apply (rule impI)
-    unfolding isin.simps
-     apply (erule FalseE)
-    apply (rule impI)
-    subgoal for y ys
-      apply (rule prod.exhaust[of y])
-      apply (raw_tactic \<open>hyp_subst_tac @{context} 1\<close>)
-      subgoal for x' \<tau>'
-        apply (rule case_split[of "x = x'"])
-         apply (raw_tactic \<open>hyp_subst_tac @{context} 1\<close>)
-        unfolding list.map map_prod_simp isin.simps bij_implies_inject[OF assms(1)]
-         apply (rule iffD2[OF if_P])
-          apply (rule refl)
-         apply (rule trans[OF _ id_apply[symmetric]])
-         apply (drule iffD1[OF if_P, rotated])
-          apply (rule refl)
-         apply assumption
-        unfolding if_not_P
-        apply (erule impE)
-         apply assumption
-        apply assumption
-        done
-      done
-    done
+    apply (rule provided)
+      apply (rule assms)+
+  apply assumption
    apply (rule Ty_App)
     apply assumption+
   apply (rule Ty_Abs)
-  unfolding fresh_def
-  apply (raw_tactic \<open>Ctr_Sugar_Tactics.unfold_thms_tac @{context} (
-    BNF_Def.set_map_of_bnf (the (BNF_Def.bnf_of @{context} "List.list"))
-  )\<close>)
-  unfolding image_comp fst_comp_map_prod[symmetric]
-  unfolding image_comp[symmetric] inj_image_mem_iff[OF bij_is_inj[OF assms(1)]]
-  apply assumption
-  unfolding list.map map_prod_simp id_def
+   apply (rule provided)
+     apply (rule assms)+
+   apply assumption
+  unfolding provided[OF assms(1,2)]
   apply assumption
   done
 
 lemma rename_Ty:
   fixes f::"'a::var_terms_pre \<Rightarrow> 'a"
   assumes "bij f" "|supp f| <o |UNIV::'a set|"
-  shows "\<Gamma> \<turnstile>\<^sub>t\<^sub>y e : \<tau>' \<longleftrightarrow> map (map_prod f id) \<Gamma> \<turnstile>\<^sub>t\<^sub>y rrename_terms f e : \<tau>'"
+  shows "\<Gamma> \<turnstile>\<^sub>t\<^sub>y e : \<tau>' \<longleftrightarrow> map_prod f id |`| \<Gamma> \<turnstile>\<^sub>t\<^sub>y vvsubst f e : \<tau>'"
   apply (rule iffI)
    apply (rule rename_Ty_aux)
      apply (rule assms)+
@@ -1409,202 +1447,891 @@ lemma rename_Ty:
     apply (rule assms)
    apply (rule supp_inv_bound)
     apply (rule assms)+
-  unfolding terms.rrename_comps[OF assms bij_imp_bij_inv[OF assms(1)] supp_inv_bound[OF assms]]
-    inv_o_simp1[OF assms(1)] terms.rrename_ids list.map_comp map_prod.comp id_o map_prod.id list.map_id
+  unfolding terms.map_comp[OF assms(2) supp_inv_bound[OF assms]]
+    inv_o_simp1[OF assms(1)] terms.map_id map_prod.comp id_o map_prod.id fset.map_comp fset.map_id
   apply assumption
   done
 
-lemma context_invariance: "\<Gamma> \<turnstile>\<^sub>t\<^sub>y e : \<tau>' \<Longrightarrow> \<forall>x\<in>FFVars_terms e. \<forall>\<tau>. (x, \<tau>) \<in> \<Gamma> \<longrightarrow> (x, \<tau>) \<in> \<Gamma>' \<Longrightarrow> \<Gamma>' \<turnstile>\<^sub>t\<^sub>y e : \<tau>'"
-proof (induction e arbitrary: \<Gamma> \<Gamma>' \<tau>' rule: TT_fresh_induct[of "{}"])
-  case Bound
-  then show ?case by (rule emp_bound)
-next
-  case (Var a)
-  then show ?case unfolding FFVars_terms_simps using Ty_Var Ty_VarE by blast
-next
-  case (App e1 e2)
-  then obtain \<tau>1 where "\<Gamma> \<turnstile>\<^sub>t\<^sub>y e1 : \<tau>1 \<rightarrow> \<tau>'" "\<Gamma> \<turnstile>\<^sub>t\<^sub>y e2 : \<tau>1" using Ty_AppE by blast
-  then have "\<Gamma>' \<turnstile>\<^sub>t\<^sub>y e1 : \<tau>1 \<rightarrow> \<tau>'" "\<Gamma>' \<turnstile>\<^sub>t\<^sub>y e2 : \<tau>1" using App by auto
-  then show ?case by (rule Ty_App)
-next
-  case (Abs x \<tau> e)
-  from Abs(3) obtain x' e' \<tau>2 f where x: "\<tau>' = (\<tau> \<rightarrow> \<tau>2)" "Abs x \<tau> e = Abs x' \<tau> e'" "(x', \<tau>)#\<Gamma> \<turnstile>\<^sub>t\<^sub>y e' : \<tau>2" "f x = x'"
-    "rrename_terms f e = e'" "bij (f::'a::var_terms_pre \<Rightarrow> 'a)" "|supp f| <o |UNIV::'a set|" "id_on (FFVars_terms (Abs x \<tau> e)) f"
-    "x' \<sharp> \<Gamma>"
-    by (smt (verit, best) Abs_inject Ty_AbsE_aux)
-  then have 1: "(f x, \<tau>)#\<Gamma> \<turnstile>\<^sub>t\<^sub>y rrename_terms f e : \<tau>2" by simp
-  have 2: "(x, \<tau>) # map (map_prod (inv f) id) \<Gamma> \<turnstile>\<^sub>t\<^sub>y e : \<tau>2"
-    apply (rule iffD2[OF rename_Ty[OF x(6,7)]])
-    unfolding list.map map_prod_simp list.map_comp map_prod.comp id_o inv_o_simp2[OF x(6)] map_prod.id list.map_id
-    unfolding id_def
-    apply (rule 1)
-    done
-  have 3: "\<forall>xa\<in>FFVars_terms e. \<forall>\<tau>'. (xa, \<tau>') \<in> (x, \<tau>) # map (map_prod (inv f) id) \<Gamma> \<longrightarrow> (xa, \<tau>') \<in> (x, \<tau>) # map (map_prod (inv f) id) \<Gamma>'"
-  proof (rule ballI, rule allI, rule impI)
-    fix y \<sigma>
-    assume a: "Set.member y (FFVars_terms e)" "(y, \<sigma>) \<in> (x, \<tau>) # map (map_prod (inv f) id) \<Gamma>"
-    have y1: "(f y, \<sigma>) \<in> (f x, \<tau>)#\<Gamma>"
-      using iffD2[OF isin_rename[OF x(6)] a(2),
-          unfolded list.map list.map_comp map_prod.comp id_o inv_o_simp2[OF x(6)] map_prod.id list.map_id map_prod_simp,
-          unfolded id_def] .
-    show "(y, \<sigma>) \<in> (x, \<tau>) # map (map_prod (inv f) id) \<Gamma>'"
-    proof (cases "x = y")
-      case True
-      then show ?thesis using a by simp
-    next
-      case False
-      then have y2: "f y = y" using x(8) a(1) unfolding id_on_def by simp
-      from False have y3: "(f y, \<sigma>) \<in> \<Gamma>" using bij_implies_inject[OF x(6)] y1 by simp
-      then have "(y, \<sigma>) \<in> \<Gamma>'" using y2 Abs(4) False a by simp
-      then have "(y, \<sigma>) \<in> map (map_prod (inv f) id) \<Gamma>'" using isin_rename[OF bij_imp_bij_inv[OF x(6)]] y2 x(6)
-        by (smt (verit) bij_betw_def inv_f_eq) 
-      then show ?thesis using False by simp
-    qed
-  qed
-  then have y4: "(x, \<tau>) # map (map_prod (inv f) id) \<Gamma>' \<turnstile>\<^sub>t\<^sub>y e : \<tau>2" using Abs(2) 2 by blast
-  have "(x', \<tau>) # \<Gamma>' \<turnstile>\<^sub>t\<^sub>y e' : \<tau>2"
-    unfolding x(4,5)[symmetric]
-    apply (rule iffD2[OF rename_Ty[OF bij_imp_bij_inv supp_inv_bound]])
-       apply (rule x(6,7))+
-    unfolding list.map map_prod_simp inv_simp1[OF x(6)] inv_o_simp1[OF x(6)] terms.rrename_ids
-      terms.rrename_comps[OF x(6,7) bij_imp_bij_inv[OF x(6)] supp_inv_bound[OF x(6,7)]]
-    unfolding id_def
-    apply (rule y4[unfolded id_def])
-    done
-  then show ?case using x(1,2,9) sorry
-qed
+definition cl :: "(('a::var_terms_pre \<times> \<tau>) fset \<Rightarrow> 'a terms \<Rightarrow> \<tau> \<Rightarrow> 'b \<Rightarrow> bool) \<Rightarrow> ('a \<times> \<tau>) fset \<Rightarrow> 'a terms \<Rightarrow> \<tau> \<Rightarrow> 'b \<Rightarrow> bool" where
+  "cl P \<Gamma> e \<tau> \<rho> \<equiv> (\<forall>f. bij f \<and> |supp f| <o |UNIV::'a set| \<longrightarrow> P (map_prod f id |`| \<Gamma>) (vvsubst f e) \<tau> \<rho>)"
 
-lemma Ty_AbsE:
-  assumes "\<Gamma> \<turnstile>\<^sub>t\<^sub>y Abs x \<tau> e : \<tau>'"
-  and "\<And>\<tau>2. \<tau>' = (\<tau> \<rightarrow> \<tau>2) \<Longrightarrow> (x, \<tau>) # \<Gamma> \<turnstile>\<^sub>t\<^sub>y e : \<tau>2 \<Longrightarrow> P"
-shows P
-proof -
-  obtain x' e' \<tau>2 f where x: "Abs x \<tau> e = Abs x' \<tau> e'" "(x', \<tau>) # \<Gamma> \<turnstile>\<^sub>t\<^sub>y e' : \<tau>2" "f x = x'" "rrename_terms f e = e'"
-    "bij (f::'a::var_terms_pre \<Rightarrow> 'a)" "|supp f| <o |UNIV::'a set|" "id_on (FFVars_terms (Abs x \<tau> e)) f" "x' \<sharp> \<Gamma>"
-    using Ty_AbsE_aux[OF assms(1)] Abs_inject by (smt (verit, best))
+lemmas clI = allI[THEN iffD2[OF meta_eq_to_obj_eq[OF cl_def]], unfolded atomize_imp[symmetric]]
 
-  obtain \<Gamma>' where "\<forall>y\<in>FFVars_terms e. \<forall>\<tau>. (y, \<tau>) \<in> \<Gamma> \<longleftrightarrow> (y, \<tau>) \<in> \<Gamma>'" by blast
-  then have "set (map fst \<Gamma>') \<subseteq> FFVars_terms e"
-    apply (induction \<Gamma>') apply (auto split!: if_splits)
-    sorry
+lemma clD:
+  fixes e::"'a::var_terms_pre terms" and f::"'a \<Rightarrow> 'a"
+assumes "cl P \<Gamma> e \<tau> \<rho>" and "bij f" "|supp f| <o |UNIV::'a set|"
+shows "P (map_prod f id |`| \<Gamma>) (vvsubst f e) \<tau> \<rho>"
+  apply (rule mp[OF spec[OF assms(1)[unfolded cl_def]]])
+  apply (rule conjI)
+   apply (rule assms)+
+  done
 
-  show ?thesis sorry
-qed
+lemma cl_ext: "cl P \<Gamma> e \<tau> \<rho> \<Longrightarrow> P \<Gamma> e \<tau> \<rho>"
+  unfolding cl_def
+  apply (erule allE)
+  apply (erule impE)
+   apply (rule conjI)
+    apply (rule bij_id)
+   apply (rule supp_id_bound)
+  unfolding map_prod.id fset.map_id terms.map_id
+  apply assumption
+  done
 
-lemma Ty_induct[consumes 1, case_names Bound Var App Abs]:
-  fixes e::"'a::var_terms_pre terms" and A::"'a set"
-  assumes "\<Gamma> \<turnstile>\<^sub>t\<^sub>y e : \<tau>"
-  and Bound: "|A| <o |UNIV::'a set|"
-  and Var: "\<And>x \<tau> \<Gamma>. (x, \<tau>) \<in> \<Gamma> \<Longrightarrow> P \<Gamma> (Var x) \<tau>"
-  and App: "\<And>\<Gamma> e1 \<tau>\<^sub>1 \<tau>\<^sub>2 e2. \<Gamma> \<turnstile>\<^sub>t\<^sub>y e1 : \<tau>\<^sub>1 \<rightarrow> \<tau>\<^sub>2 \<Longrightarrow> P \<Gamma> e1 (\<tau>\<^sub>1 \<rightarrow> \<tau>\<^sub>2) \<Longrightarrow> \<Gamma> \<turnstile>\<^sub>t\<^sub>y e2 : \<tau>\<^sub>1 \<Longrightarrow> P \<Gamma> e2 \<tau>\<^sub>1 \<Longrightarrow> P \<Gamma> (App e1 e2) \<tau>\<^sub>2"
-  and Abs: "\<And>x \<Gamma> \<tau> e \<tau>\<^sub>2. x \<notin> A \<Longrightarrow> x \<sharp> \<Gamma> \<Longrightarrow> (x, \<tau>) # \<Gamma> \<turnstile>\<^sub>t\<^sub>y e : \<tau>\<^sub>2 \<Longrightarrow> P ((x, \<tau>) # \<Gamma>) e \<tau>\<^sub>2 \<Longrightarrow> P \<Gamma> (Abs x \<tau> e) (\<tau> \<rightarrow> \<tau>\<^sub>2)"
-shows "P \<Gamma> e \<tau>"
-  apply (rule Ty.induct)
-     apply (rule assms(1))
-    apply (rule Var)
-    apply assumption
-   apply (rule App)
+lemma cl_vvsubst:
+  fixes e::"'a::var_terms_pre terms"
+  assumes f: "bij f" "|supp f| <o |UNIV::'a set|" and cl: "cl P \<Gamma> e \<tau> \<rho>"
+  shows "cl P (map_prod f id |`| \<Gamma>) (vvsubst f e) \<tau> \<rho>"
+  unfolding cl_def
+  apply (rule allI impI)+
+  apply (erule conjE)
+  unfolding fset.map_comp terms.map_comp[OF f(2)] map_prod.comp id_o
+  apply (rule clD[OF cl])
+   apply (rule bij_comp)
+    apply (rule f)
+   apply assumption
+  apply (rule supp_comp_bound)
+    apply (rule f)
+   apply assumption
+  apply (rule cinfinite_imp_infinite[OF terms_pre.UNIV_cinfinite])
+  done
+
+lemma cl_cl: "cl (cl P) = cl P"
+  unfolding cl_def
+  apply (rule ext)+
+  apply (rule iffI)
+   apply (rule allI)
+   apply (rule impI)
+   apply (erule allE)
+   apply (erule conjE)
+   apply (erule impE)
+    apply (rule conjI)
+     apply assumption+
+   apply (erule allE)
+   apply (erule impE)
+    apply (rule conjI)
+     apply (rule bij_id)
+    apply (rule supp_id_bound)
+  unfolding map_prod.id fset.map_id terms.map_id
+   apply assumption
+  apply (rule allI impI)+
+  apply (erule allE conjE)+
+  apply (erule impE)
+   defer
+  unfolding fset.map_comp map_prod.comp id_o terms.map_comp
+   apply assumption
+  apply (rule conjI)
+   apply (rule bij_comp)
+    apply assumption+
+  apply (rule supp_comp_bound)
+    apply assumption+
+  apply (rule cinfinite_imp_infinite[OF terms_pre.UNIV_cinfinite])
+  done
+
+lemma TT_inject: "(terms_ctor a = terms_ctor b) = (\<exists>(f::'a::var_terms_pre \<Rightarrow> 'a). bij f \<and> |supp f| <o |UNIV::'a set|
+  \<and> id_on (\<Union>(FFVars_terms ` set3_terms_pre a) - set2_terms_pre a) f \<and> map_terms_pre id f (vvsubst f) id a = b)"
+  unfolding terms.TT_injects0 conj_assoc[symmetric]
+  apply (rule ex_cong)
+  apply (erule conjE)+
+  unfolding terms_vvsubst_rrename
+  apply (rule refl)
+  done
+
+(*no_notation extend ("(_,_:_)")*)
+
+lemma ex_avoiding_bij:
+  fixes f :: "'a \<Rightarrow> 'a" and I D A :: "'a set"
+  assumes  "|supp f| <o |UNIV :: 'a set|" "bij f" "infinite (UNIV :: 'a set)"
+    "|I| <o |UNIV :: 'a set|" "id_on I f"
+    "|D| <o |UNIV :: 'a set|" "D \<inter> A = {}" "|A| <o |UNIV :: 'a set|"
+  shows "\<exists>(g::'a \<Rightarrow> 'a). bij g \<and> |supp g| <o |UNIV::'a set| \<and> imsupp g \<inter> A = {} \<and>
+    (\<forall>a. a \<in> (imsupp f - A) \<union> D \<and> f a \<notin> A \<longrightarrow> g a = f a) \<and> id_on I g"
+  apply (rule exI[of _ "avoiding_bij f I D A"])
+  apply (rule conjI avoiding_bij assms)+
+  done
+
+lemma id_on_empty: "id_on {} f"
+  unfolding id_on_def by simp
+lemma disjoint_single: "{x} \<inter> A = {} \<longleftrightarrow> x \<notin> A"
+  by simp
+
+lemma Ty_fresh_induct_param:
+  fixes K::"'p \<Rightarrow> 'a::var_terms_pre set" and e::"'a terms"
+  assumes bound: "\<forall>\<rho>. |K \<rho>| <o |UNIV::'a set|" and x: "\<Gamma> \<turnstile>\<^sub>t\<^sub>y e : \<tau>"
+    and Ty_Var: "\<And>x \<tau> \<Gamma> \<rho>. (x, \<tau>) |\<in>| \<Gamma> \<Longrightarrow> P \<Gamma> (Var x) \<tau> \<rho>"
+    and Ty_App: "\<And>\<Gamma> e1 \<tau>\<^sub>1 \<tau>\<^sub>2 e2 \<rho>. \<Gamma> \<turnstile>\<^sub>t\<^sub>y e1 : \<tau>\<^sub>1 \<rightarrow> \<tau>\<^sub>2 \<Longrightarrow> \<forall>\<rho>. P \<Gamma> e1 (\<tau>\<^sub>1 \<rightarrow> \<tau>\<^sub>2) \<rho>
+      \<Longrightarrow> \<Gamma> \<turnstile>\<^sub>t\<^sub>y e2 : \<tau>\<^sub>1 \<Longrightarrow> \<forall>\<rho>. P \<Gamma> e2 \<tau>\<^sub>1 \<rho> \<Longrightarrow> P \<Gamma> (App e1 e2) \<tau>\<^sub>2 \<rho>"
+    and Ty_Abs: "\<And>x \<Gamma> \<tau> e \<tau>\<^sub>2 \<rho>. x \<notin> K \<rho> \<Longrightarrow> x \<sharp> \<Gamma> \<Longrightarrow> extend \<Gamma> x \<tau> \<turnstile>\<^sub>t\<^sub>y e : \<tau>\<^sub>2 \<Longrightarrow> \<forall>\<rho>. P (extend \<Gamma> x \<tau>) e \<tau>\<^sub>2 \<rho> \<Longrightarrow> P \<Gamma> (Abs x \<tau> e) (\<tau> \<rightarrow> \<tau>\<^sub>2) \<rho>"
+  shows "\<forall>\<rho>. P \<Gamma> e \<tau> \<rho>"
+  apply (rule allI)
+  apply (rule cl_ext[of P])
+  apply (rule spec[OF Ty.induct[OF x, of "\<lambda>\<Gamma> e \<tau>. \<forall>\<rho>. cl P \<Gamma> e \<tau> \<rho>"]])
+
+  (* Nonbinding case *)
+    apply (rule allI)
+    apply (rule clI)
+    apply (erule conjE)
+  unfolding vvsubst_simps
+    apply (rule Ty_Var)
+    apply (rule provided)
       apply assumption+
-  subgoal for x \<Gamma> \<tau> e \<tau>2
+  (* And again *)
+  apply (rule allI)
+   apply (rule clI)
+   apply (erule conjE)
+  unfolding vvsubst_simps
+   apply (rule Ty_App)
+      apply (assumption | (rule allI, (erule allE)+, rule clD[of P]) | rule iffD1[OF rename_Ty])+
+  (* binding case *)
+  subgoal for \<rho> x \<Gamma> \<tau> e \<tau>2
+  apply (rule allI)
+  apply (rule clI[of P])
+    apply (erule conjE)
+    subgoal for \<rho> f
+      apply (rule exE[OF Abs_avoid])
+       apply (rule terms_pre.Un_bound)
+      apply (rule terms_pre.Un_bound)
+        apply (rule iffD2[OF imsupp_supp_bound[OF cinfinite_imp_infinite[OF terms_pre.UNIV_cinfinite]]])
+        apply assumption
+        apply (rule spec[OF bound])
+       apply (rule terms_pre.UNION_bound)
+      apply (rule ordLess_ordLeq_trans[of "|fset \<Gamma>|"])
+apply (raw_tactic \<open>resolve_tac @{context} (
+        BNF_Def.set_bd_of_bnf (the (BNF_Def.bnf_of @{context} "FSet.fset"))
+      ) 1\<close>)
+        apply (rule terms.var_large)
+       apply (rule ordLess_ordLeq_trans[of "|Basic_BNFs.fsts _|"])
+      apply (raw_tactic \<open>resolve_tac @{context} (
+        BNF_Def.set_bd_of_bnf (the (BNF_Def.bnf_of @{context} @{type_name prod}))
+      ) 1\<close>)
+      apply (rule terms.var_large)
+     apply (erule exE conjE)+
 
-(*
-    apply (rule exE[OF Abs_avoid[of _ x \<tau> e]])
-     apply (rule terms.Un_bound)
-      apply (rule Bound)
-    apply (rule ordLess_ordLeq_trans)
-    apply (raw_tactic \<open>resolve_tac @{context} (
-      BNF_Def.set_bd_of_bnf (the (BNF_Def.bnf_of @{context} "List.list"))
-    ) 1\<close>)
-    unfolding Un_iff de_Morgan_disj
-    apply (rule terms_pre.var_large)
-    apply (erule exE conjE)+
-    apply (rule iffD2[OF arg_cong3[OF refl _ refl, of _ _ P]])
-     apply assumption
-    unfolding Abs_inject
-    apply (erule exE conjE)+
-    apply (rule iffD2[OF arg_cong3[OF _ refl refl, of _ _ P]])
-    defer
-    apply (raw_tactic \<open>hyp_subst_tac @{context} 1\<close>)
-    apply (rule Abs)
-       apply assumption
-    unfolding fresh_def
+       apply (rule iffD2[OF fun_cong[of _ _ \<rho>]])
+        apply (rule arg_cong3[OF refl _ refl, of _ _ P])
+        apply (rule arg_cong2[OF refl, of _ _ vvsubst])
+        apply assumption
+      unfolding Un_iff de_Morgan_disj
+       apply (erule conjE)+
+      unfolding vvsubst_simps
+       apply (rule Ty_Abs)
+          apply assumption
+         apply (rule iffD2[OF arg_cong2[OF _ refl, of _ _ fresh]])
+          apply (rule not_in_imsupp_same[symmetric])
+          apply assumption
+         apply (rule provided)
+          apply assumption+
+
+        apply (unfold Abs_inject)[1]
+        apply (erule exE conjE)+
+        apply hypsubst
+        apply (rule exE[OF ex_avoiding_bij])
+                apply (rotate_tac -3)
+                apply assumption
+               apply assumption
+              apply (rule cinfinite_imp_infinite[OF terms_pre.UNIV_cinfinite])
+             apply (rule emp_bound)
+            apply (rule id_on_empty)
+           apply (rule singl_bound[of "x"])
+          apply (rule iffD2[OF disjoint_single])
+          apply (rule provided)
+             apply assumption+
+      apply (rule terms_pre.UNION_bound)
+         apply (rule ordLess_ordLeq_trans)
+      apply (raw_tactic \<open>resolve_tac @{context} (
+        BNF_Def.set_bd_of_bnf (the (BNF_Def.bnf_of @{context} "FSet.fset"))
+      ) 1\<close>)
+          apply (rule terms.var_large)
+         apply (rule ordLess_ordLeq_trans)
+      apply (raw_tactic \<open>resolve_tac @{context} (
+        BNF_Def.set_bd_of_bnf (the (BNF_Def.bnf_of @{context} @{type_name prod}))
+      ) 1\<close>)
+      apply (rule terms.var_large)
+        apply (erule conjE allE)+
+        apply (erule impE)
+         prefer 2
+         apply (rule iffD2[OF arg_cong2[of _ _ _ _ fresh]])
+          apply (rule sym)
+           apply assumption
+          prefer 2
+          apply (drule provided(2)[rotated -1])
+            apply (rotate_tac -6)
+            apply assumption+
+         apply (rule iffD1[OF fun_cong[OF fun_cong [OF fset.rel_eq]]])
+         apply (rule iffD2[OF fset.rel_map(2)])
+         apply (rule fset.rel_refl_strong)
+         apply (rule iffD1[OF fun_cong[OF fun_cong[OF prod.rel_eq]]])
+         apply (rule iffD2[OF prod.rel_map(2)])
+         apply (rule prod.rel_refl_strong)
+          apply (rule not_in_imsupp_same[symmetric])
+      apply (drule trans[OF Int_commute])
+          apply (unfold disjoint_iff)[1]
+          apply (erule allE)
+          apply (erule impE)
+           apply (rule UN_I)
+            apply assumption+
+      apply (rule id_apply[symmetric])
+
+         apply (rule conjI)
+          apply (rule UnI2)
+         apply (rule singletonI)
+        apply assumption
+
+       apply (rule iffD2[OF arg_cong3[OF _ refl refl, of _ _ Ty]])
+        apply (rule arg_cong3[OF refl _ refl, of _ _ extend])
+        apply (rule not_in_imsupp_same[symmetric])
+        apply assumption
+      unfolding provided(3)[symmetric]
+       apply (rule iffD1[OF rename_Ty])
+      apply assumption+
+
+
+       apply (unfold Abs_inject)[1]
+       apply (erule exE conjE)+
+       apply hypsubst
+       apply (unfold terms_vvsubst_rrename[symmetric])[1]
+       apply (rule exE[OF ex_avoiding_bij])
+               apply (rotate_tac -3)
+               apply assumption
+              apply assumption
+             apply (rule cinfinite_imp_infinite[OF terms_pre.UNIV_cinfinite])
+            prefer 2
+            apply assumption
+           apply (rule terms.card_of_FFVars_bounds)
+          apply (rule singl_bound[of "x"])
+         apply (rule iffD2[OF disjoint_single])
+         apply (rule provided)
+            apply assumption+
+        apply (rule terms_pre.UNION_bound)
+         apply (rule ordLess_ordLeq_trans)
+      apply (raw_tactic \<open>resolve_tac @{context} (
+        BNF_Def.set_bd_of_bnf (the (BNF_Def.bnf_of @{context} "FSet.fset"))
+      ) 1\<close>)
+          apply (rule terms.var_large)
+         apply (rule ordLess_ordLeq_trans)
+      apply (raw_tactic \<open>resolve_tac @{context} (
+        BNF_Def.set_bd_of_bnf (the (BNF_Def.bnf_of @{context} @{type_name prod}))
+      ) 1\<close>)
+        apply (rule terms.var_large)
+       apply (erule conjE)+
+       apply (rotate_tac -2)
+      apply (erule allE)
+       apply (rule iffD2[OF arg_cong3[OF _ _ refl, of _ _ _ _ Ty]])
+         apply (rule arg_cong3[OF refl _ refl, of _ _ extend])
+         apply (rule sym)
+         apply (erule impE)
+          apply (rule conjI)
+           apply (rule UnI2)
+           apply (rule singletonI)
+          apply assumption
+         apply assumption
+        apply (rule terms.map_cong0)
+          apply assumption
+         apply (rotate_tac -4)
       apply assumption
-    unfolding fresh_def[symmetric]
-     apply (drule rename_Ty[rotated -1])
+        apply (unfold FFVars_terms_simps)[1]
+      subgoal for y e' f' g z
+        apply (rule case_split[of "z \<in> {x}"])
+          apply (drule singletonD)
+         apply hypsubst_thin
+         apply (erule impE)
+          apply (rule conjI)
+           apply (rule UnI2)
+           apply (rule singletonI)
+          apply assumption
+         apply (rule sym)
+         apply assumption
+        apply (drule id_onD)
+         apply (rule DiffI)
+          apply assumption
+         apply assumption
+        apply (drule id_onD)
+         apply (rule DiffI)
+          apply assumption
+         apply assumption
+        apply (rule trans)
+         apply assumption
+        apply (rule sym)
+        apply assumption
+        done
+      subgoal for y e' f' g
+       apply (rule iffD2[OF arg_cong3[OF _ refl refl, of _ _ Ty]])
+      apply (rule trans)
+        apply (rule arg_cong3[OF _ refl refl, of _ _ extend])
+          prefer 2
+          apply (rule provided(3)[symmetric, of "g"])
+        apply assumption+
+      apply (rule iffD1[OF fun_cong[OF fun_cong [OF fset.rel_eq]]])
+         apply (rule iffD2[OF fset.rel_map(2)])
+         apply (rule fset.rel_refl_strong)
+         apply (rule iffD1[OF fun_cong[OF fun_cong[OF prod.rel_eq]]])
+         apply (rule iffD2[OF prod.rel_map(2)])
+         apply (rule prod.rel_refl_strong)
+          apply (drule trans[OF Int_commute])
+          apply (unfold disjoint_iff)[1]
+          apply (erule allE)+
+          apply (rotate_tac -1)
+          apply (erule impE)
+           apply (rule UN_I)
+            apply assumption
+           apply assumption
+          apply (rule not_in_imsupp_same[symmetric])
+          apply assumption
+         apply (rule id_apply[symmetric])
+        apply (rule iffD1[OF rename_Ty])
+          apply assumption+
+        done
+      apply (rule allI)
+      apply (rule iffD2[OF fun_cong[of "P _ _ _"]])
+       apply (rule arg_cong3[OF _ refl refl])
+       apply (rule arg_cong3[OF refl _ refl, of _ _ extend])
+       apply (rule not_in_imsupp_same[symmetric])
+       apply assumption
+      unfolding provided(3)[symmetric]
+      apply (rule clD[of P, rotated])
+        apply assumption+
+      apply (unfold Abs_inject)
+      apply (erule exE conjE)+
+      apply hypsubst_thin
+      apply (unfold terms_vvsubst_rrename[symmetric])
+      apply (rule exE[OF ex_avoiding_bij])
+              apply (rotate_tac -3)
+              apply assumption
+      apply assumption
+            apply (rule cinfinite_imp_infinite[OF terms_pre.UNIV_cinfinite])
+           prefer 2
+           apply assumption
+          apply (rule terms.card_of_FFVars_bounds)
+         apply (rule singl_bound)
+        apply (rule iffD2[OF disjoint_single])
+      apply (rule provided)
+        apply assumption+
+      apply (rule terms_pre.UNION_bound)
+         apply (rule ordLess_ordLeq_trans)
+      apply (raw_tactic \<open>resolve_tac @{context} (
+        BNF_Def.set_bd_of_bnf (the (BNF_Def.bnf_of @{context} "FSet.fset"))
+      ) 1\<close>)
+          apply (rule terms.var_large)
+         apply (rule ordLess_ordLeq_trans)
+      apply (raw_tactic \<open>resolve_tac @{context} (
+        BNF_Def.set_bd_of_bnf (the (BNF_Def.bnf_of @{context} @{type_name prod}))
+      ) 1\<close>)
+       apply (rule terms.var_large)
+      apply (erule conjE)+
+      apply (rotate_tac -2)
+      apply (erule allE)
+      apply (rule iffD2[OF fun_cong[of "cl _ _ _ _"]])
+       apply (rule fun_cong[of "cl _ _ _"])
+       apply (rule arg_cong3[OF refl _ _, of _ _ _ _ cl])
+        apply (rule arg_cong3[OF _ _ refl, of _ _ _ _ extend])
+      defer
+        apply (erule impE)
+         prefer 2
+         apply (rule sym)
+         apply assumption
+        apply (rule conjI)
+         apply (rule UnI2)
+         apply (rule singletonI)
+        apply assumption
+       apply (rule terms.map_cong0)
+         apply assumption
+        apply (rotate_tac -4)
+      apply assumption+
+      subgoal for y e' \<rho> f' g z
+        apply (rule case_split[of "z \<in> {x}"])
+         apply (drule singletonD)
+         apply hypsubst_thin
+         apply (erule impE)
+          apply (rule conjI)
+           apply (rule UnI2)
+           apply (rule singletonI)
+          apply assumption
+         apply (rule sym)
+         apply assumption
+        unfolding FFVars_terms_simps
+        apply (drule id_onD, rule DiffI, assumption+)+
+        apply (rule trans)
+         apply assumption
+        apply (rule sym)
+        apply assumption
+        done
+       apply (rule iffD2[OF fun_cong[of "cl _ _ _ _"]])
+        apply (rule fun_cong[of "cl _ _ _"])
+        apply (rule arg_cong3[OF refl _ refl, of _ _ cl])
+        apply (rule provided(3)[symmetric, of _ x])
+         apply assumption+
+       apply (rule cl_vvsubst)
+         apply assumption+
+       apply (erule allE)
+       apply assumption
+  apply (rule iffD1[OF fun_cong[OF fun_cong [OF fset.rel_eq]]])
+         apply (rule iffD2[OF fset.rel_map(2)])
+         apply (rule fset.rel_refl_strong)
+         apply (rule iffD1[OF fun_cong[OF fun_cong[OF prod.rel_eq]]])
+         apply (rule iffD2[OF prod.rel_map(2)])
+         apply (rule prod.rel_refl_strong)
+          apply (drule trans[OF Int_commute])
+       apply (unfold disjoint_iff)[1]
+       apply (rule not_in_imsupp_same[symmetric])
+       apply (erule allE)+
+       apply (rotate_tac -1)
+       apply (erule impE)
+        apply (rule UN_I)
+         apply assumption+
+      apply (rule id_apply[symmetric])
+      done
+  done
+  done
+
+lemma Ty_fresh_induct:
+  fixes A::"'a::var_terms_pre set" and e::"'a terms"
+  assumes "|A| <o |UNIV::'a set|" and x: "\<Gamma> \<turnstile>\<^sub>t\<^sub>y e : \<tau>"
+    and Ty_Var: "\<And>x \<tau> \<Gamma>. (x, \<tau>) |\<in>| \<Gamma> \<Longrightarrow> P \<Gamma> (Var x) \<tau>"
+    and Ty_App: "\<And>\<Gamma> e1 \<tau>\<^sub>1 \<tau>\<^sub>2 e2. \<Gamma> \<turnstile>\<^sub>t\<^sub>y e1 : \<tau>\<^sub>1 \<rightarrow> \<tau>\<^sub>2 \<Longrightarrow> P \<Gamma> e1 (\<tau>\<^sub>1 \<rightarrow> \<tau>\<^sub>2) \<Longrightarrow> \<Gamma> \<turnstile>\<^sub>t\<^sub>y e2 : \<tau>\<^sub>1
+      \<Longrightarrow> P \<Gamma> e2 \<tau>\<^sub>1 \<Longrightarrow> P \<Gamma> (App e1 e2) \<tau>\<^sub>2"
+    and Ty_Abs: "\<And>x \<Gamma> \<tau> e \<tau>\<^sub>2. x \<notin> A \<union> fst ` fset \<Gamma> \<union> FFVars_terms (Abs x \<tau> e) \<Longrightarrow> x \<sharp> \<Gamma> \<Longrightarrow> \<Gamma>,x:\<tau> \<turnstile>\<^sub>t\<^sub>y e : \<tau>\<^sub>2 \<Longrightarrow> P \<Gamma>,x:\<tau> e \<tau>\<^sub>2 \<Longrightarrow> P \<Gamma> (Abs x \<tau> e) (\<tau> \<rightarrow> \<tau>\<^sub>2)"
+  shows "P \<Gamma> e \<tau>"
+  apply (rule mp[OF spec[OF Ty_fresh_induct_param[of "\<lambda>\<rho>. case \<rho> of (\<Gamma>, e) \<Rightarrow> A \<union> fst ` fset \<Gamma> \<union> FFVars_terms e" _ _ _ "\<lambda>\<Gamma> e \<tau> \<rho>. \<rho> = (\<Gamma>, e) \<longrightarrow> P \<Gamma> e \<tau>"]]])
+       apply (rule allI)
+  subgoal for x
+    apply (rule prod.exhaust[of x])
+    apply hypsubst_thin
+    unfolding prod.case
+    apply (rule terms.Un_bound)
+     apply (rule terms.Un_bound)
+    apply (rule assms(1))
+     apply (rule ordLeq_ordLess_trans[OF card_of_image])
+     apply (rule ordLess_ordLeq_trans)
+      apply (raw_tactic \<open>resolve_tac @{context} (BNF_Def.set_bd_of_bnf (the (BNF_Def.bnf_of @{context} "FSet.fset"))) 1\<close>)
+     apply (rule terms_pre.var_large)
+    apply (rule terms.set_bd_UNIV)
+    done
+      apply (rule x)
+     apply (rule impI)
+     apply (rule Ty_Var)
+     apply assumption
+    apply (rule impI)
+  apply (erule allE, erule impE, rule refl)+
+    apply (rule Ty_App)
        apply assumption+
-    unfolding list.map map_prod_simp id_def
-    unfolding id_def[symmetric]
-*)
+   apply (rule impI)
+   apply (rule Ty_Abs)
+  subgoal for x \<Gamma> \<tau> e \<tau>2 y
+    apply (rule prod.exhaust[of y])
+    apply (raw_tactic \<open>hyp_subst_tac @{context} 1\<close>)
+    unfolding prod.case Un_iff de_Morgan_disj
+    apply (erule conjE)+
+    apply (rule conjI)+
+     apply assumption+
+    done
+     apply assumption+
+   apply (erule allE)
+   apply (erule impE)
+    apply (rule refl)
+   apply assumption
+  apply (rule refl)
+  done
+
+lemmas Ty_induct_strong = Ty_fresh_induct[OF emp_bound, unfolded Un_empty_left]
+
+inductive_cases
+  Ty_VarE[elim]: "\<Gamma> \<turnstile>\<^sub>t\<^sub>y Var x : \<tau>"
+  and Ty_AppE[elim]: "\<Gamma> \<turnstile>\<^sub>t\<^sub>y App e1 e2 : \<tau>\<^sub>2"
+print_theorems
+
+lemma provided_strong:
+  fixes f::"'a::var_terms_pre \<Rightarrow> 'a" and \<Gamma>::"('a \<times> \<tau>) fset"
+  shows "bij f \<Longrightarrow> |supp f| <o |UNIV::'a set| \<Longrightarrow> x \<sharp> \<Gamma> \<longleftrightarrow> f x \<sharp> map_prod f id |`| \<Gamma>"
+  apply (rule iffI)
+   apply (rule provided)
+  apply assumption+
+  apply (drule provided[rotated -1])
+    apply (rule bij_imp_bij_inv)
+  apply assumption
+  apply (rule supp_inv_bound)
+  apply assumption+
+  unfolding inv_simp1 fset.map_comp comp_def prod.map_comp id_def
+  unfolding id_def[symmetric] prod.map_id fset.map_id
+  apply assumption
+  done
+
+(* automate with binder_inductive_cases *)
+lemma Ty_AbsE:
+  fixes e::"'a::var_terms_pre terms" and A::"'a set"
+  assumes "\<Gamma> \<turnstile>\<^sub>t\<^sub>y Abs x \<tau>\<^sub>1 e : \<tau>" "|A| <o |UNIV::'a set|"
+    and "\<And>y e' \<tau>' \<tau>\<^sub>2. y \<notin> A \<Longrightarrow> Abs x \<tau>\<^sub>1 e = Abs y \<tau>' e' \<Longrightarrow> \<tau> = (\<tau>' \<rightarrow> \<tau>\<^sub>2) \<Longrightarrow> y \<sharp> \<Gamma> \<Longrightarrow> \<Gamma>,y:\<tau>' \<turnstile>\<^sub>t\<^sub>y e' : \<tau>\<^sub>2 \<Longrightarrow> P"
+  shows P
+  apply (rule mp[OF Ty_fresh_induct[OF assms(2,1), of "\<lambda>\<Gamma>' e' \<tau>'. \<Gamma>' = \<Gamma> \<and> e' = Abs x \<tau>\<^sub>1 e \<and> \<tau>' = \<tau> \<longrightarrow> P"]])
+     apply (rule impI, (erule conjE)+, rotate_tac -2, drule cnf.clause2raw_notE, rule terms_distinct, erule FalseE)+
+   apply (rule impI)
+   apply (erule conjE)+
+   apply hypsubst
+  unfolding Un_iff de_Morgan_disj
+   apply (erule conjE)+
+   apply (rule assms(3))
+       apply assumption
+      apply (rule sym)
+      apply assumption+
+  apply (rule conjI refl)+
+  done
+lemma Ty_AbsE':
+  assumes "\<Gamma> \<turnstile>\<^sub>t\<^sub>y Abs x \<tau>\<^sub>1 e : \<tau>" "x \<notin> \<Union>(Basic_BNFs.fsts ` fset \<Gamma>)"
+and "\<And>\<tau>\<^sub>2. \<tau> = (\<tau>\<^sub>1 \<rightarrow> \<tau>\<^sub>2) \<Longrightarrow> x \<sharp> \<Gamma> \<Longrightarrow> \<Gamma>,x:\<tau>\<^sub>1 \<turnstile>\<^sub>t\<^sub>y e : \<tau>\<^sub>2 \<Longrightarrow> P"
+shows "P"
+  apply (rule Ty_AbsE)
+    apply (rule assms(1))
+  apply (rule terms_pre.UNION_bound)
+         apply (rule ordLess_ordLeq_trans)
+      apply (raw_tactic \<open>resolve_tac @{context} (
+        BNF_Def.set_bd_of_bnf (the (BNF_Def.bnf_of @{context} "FSet.fset"))
+      ) 1\<close>)
+          apply (rule terms.var_large)
+         apply (rule ordLess_ordLeq_trans)
+      apply (raw_tactic \<open>resolve_tac @{context} (
+        BNF_Def.set_bd_of_bnf (the (BNF_Def.bnf_of @{context} @{type_name prod}))
+      ) 1\<close>)
+   apply (rule terms.var_large)
+
+  unfolding Abs_inject
+  apply (erule exE conjE)+
+  apply hypsubst
+
+  apply (rule exE[OF ex_avoiding_bij])
+          apply assumption+
+        apply (rule cinfinite_imp_infinite[OF terms_pre.UNIV_cinfinite])
+       apply (rule terms.set_bd_UNIV)
+      apply assumption
+     apply (rule singl_bound)
+    apply (rule iffD2[OF disjoint_single])
+  apply (rule assms(2))
+apply (rule terms_pre.UNION_bound)
+         apply (rule ordLess_ordLeq_trans)
+      apply (raw_tactic \<open>resolve_tac @{context} (
+        BNF_Def.set_bd_of_bnf (the (BNF_Def.bnf_of @{context} "FSet.fset"))
+      ) 1\<close>)
+          apply (rule terms.var_large)
+         apply (rule ordLess_ordLeq_trans)
+      apply (raw_tactic \<open>resolve_tac @{context} (
+        BNF_Def.set_bd_of_bnf (the (BNF_Def.bnf_of @{context} @{type_name prod}))
+      ) 1\<close>)
+   apply (rule terms.var_large)
+  apply (erule conjE)+
+
+  apply (rule assms(3))
+    apply assumption
+   apply (drule iffD1[OF arg_cong2[of _ _ _ _ "\<lambda>a b. a \<sharp> b"], rotated -1])
+     apply (erule allE)
+     apply (erule impE)
+      prefer 2
+      apply (rule sym)
+      apply assumption
+     apply (rule conjI)
+      apply (rule UnI2)
+      apply (rule singletonI)
+     apply assumption
+    prefer 2
+    apply (rule iffD2[OF provided_strong])
+      apply (rotate_tac -6)
+      apply assumption+
+ apply (rule iffD1[OF fun_cong[OF fun_cong [OF fset.rel_eq]]])
+         apply (rule iffD2[OF fset.rel_map(2)])
+         apply (rule fset.rel_refl_strong)
+         apply (rule iffD1[OF fun_cong[OF fun_cong[OF prod.rel_eq]]])
+         apply (rule iffD2[OF prod.rel_map(2)])
+         apply (rule prod.rel_refl_strong)
+  apply (drule trans[OF Int_commute])
+       apply (unfold disjoint_iff)[1]
+    apply (rule not_in_imsupp_same[symmetric])
+    apply (erule allE)+
+    apply (rotate_tac -1)
+    apply (erule impE)
+     apply (rule UN_I)
+      apply assumption+
+   apply (rule id_apply[symmetric])
+
+  apply (rule iffD2[OF rename_Ty])
+    apply (rotate_tac -5)
+    apply assumption+
+  unfolding provided
+  apply (rule iffD2[OF arg_cong3[OF _ _ refl, of _ _ _ _ Ty], rotated -1])
+    apply assumption
+   apply (rule arg_cong3[OF _ _ refl, of _ _ _ _ extend])
+  apply (rule sym)
+apply (rule iffD1[OF fun_cong[OF fun_cong [OF fset.rel_eq]]])
+         apply (rule iffD2[OF fset.rel_map(2)])
+         apply (rule fset.rel_refl_strong)
+         apply (rule iffD1[OF fun_cong[OF fun_cong[OF prod.rel_eq]]])
+         apply (rule iffD2[OF prod.rel_map(2)])
+         apply (rule prod.rel_refl_strong)
+  apply (drule trans[OF Int_commute])
+       apply (unfold disjoint_iff)[1]
+     apply (rule not_in_imsupp_same[symmetric])
+     apply (rotate_tac -1)
+     apply (erule allE)
+     apply (erule impE)
+      apply (rule UN_I)
+       apply assumption+
+    apply (rule id_apply[symmetric])
+   apply (erule allE)
+   apply (erule impE)
+    prefer 2
+    apply assumption
+   apply (rule conjI)
+    apply (rule UnI2)
+    apply (rule singletonI)
+   apply assumption
+  apply (rule trans[rotated])
+   apply (rule fun_cong[OF terms_vvsubst_rrename])
+    apply assumption+
+  apply (rule terms.map_cong0)
+    apply assumption+
+  subgoal for y e' \<tau>' \<tau>2 f g z
+    apply (rule case_split[of "z \<in> {x}"])
+     apply (drule singletonD)
+     apply hypsubst
+     apply (erule allE)
+     apply (erule impE)
+      prefer 2
+      apply assumption
+     apply (rule conjI)
+      apply (rule UnI2)
+      apply (rule singletonI)
+     apply assumption
+    unfolding FFVars_terms_simps
+    apply (drule id_onD, rule DiffI, assumption+)+
+    apply (rule trans)
+     apply assumption
+    apply (rule sym)
+    apply assumption
+    done
+  done
+
+(* TODO: automate with binder_induction method *)
+lemma context_invariance_induct[consumes 2, case_names Var App Abs]:
+  fixes e::"'a::var_terms_pre terms"
+  assumes "\<Gamma> \<turnstile>\<^sub>t\<^sub>y e : \<tau>" "\<forall>x\<in>FFVars_terms e. \<forall>\<tau>. (x, \<tau>) |\<in>| \<Gamma> \<longrightarrow> (x, \<tau>) |\<in>| \<Gamma>'"
+and Var: "\<And>(x::'a) \<tau> \<Gamma> \<Gamma>'. \<lbrakk> (x, \<tau>) |\<in>| \<Gamma> ; \<forall>x\<in>FFVars_terms (Var x). \<forall>\<tau>. (x, \<tau>) |\<in>| \<Gamma> \<longrightarrow> (x, \<tau>) |\<in>| \<Gamma>' \<rbrakk> \<Longrightarrow> \<Gamma>' \<turnstile>\<^sub>t\<^sub>y (Var x) : \<tau>"
+and App: "\<And>\<Gamma> \<Gamma>' (e1::'a terms) \<tau>\<^sub>1 \<tau>\<^sub>2 e2. \<lbrakk> \<Gamma> \<turnstile>\<^sub>t\<^sub>y e1 : \<tau>\<^sub>1 \<rightarrow> \<tau>\<^sub>2 ; \<Gamma> \<turnstile>\<^sub>t\<^sub>y e2 : \<tau>\<^sub>1 ; \<And>\<Gamma>'. \<forall>x\<in>FFVars_terms e1. \<forall>\<tau>. (x, \<tau>) |\<in>| \<Gamma> \<longrightarrow> (x, \<tau>) |\<in>| \<Gamma>' \<Longrightarrow> \<Gamma>' \<turnstile>\<^sub>t\<^sub>y e1 : \<tau>\<^sub>1 \<rightarrow> \<tau>\<^sub>2 ; \<And>\<Gamma>'. \<forall>x\<in>FFVars_terms e2. \<forall>\<tau>. (x, \<tau>) |\<in>| \<Gamma> \<longrightarrow> (x, \<tau>) |\<in>| \<Gamma>' \<Longrightarrow> \<Gamma>' \<turnstile>\<^sub>t\<^sub>y e2 : \<tau>\<^sub>1 ; \<forall>x\<in>FFVars_terms (App e1 e2). \<forall>\<tau>. (x, \<tau>) |\<in>| \<Gamma> \<longrightarrow> (x, \<tau>) |\<in>| \<Gamma>' \<rbrakk> \<Longrightarrow> \<Gamma>' \<turnstile>\<^sub>t\<^sub>y (App e1 e2) : \<tau>\<^sub>2"
+and Abs: "\<And>(x::'a) \<Gamma> \<Gamma>' \<tau> e \<tau>\<^sub>2. \<lbrakk> x \<notin> \<Union>(Basic_BNFs.fsts ` fset \<Gamma>) \<union> \<Union>(Basic_BNFs.fsts ` fset \<Gamma>') \<union> FFVars_terms (Abs x \<tau> e) ; x \<sharp> \<Gamma> ; \<Gamma>,x:\<tau> \<turnstile>\<^sub>t\<^sub>y e : \<tau>\<^sub>2 ; \<And>\<Gamma>'. \<forall>y\<in>FFVars_terms e. \<forall>\<tau>'. (y, \<tau>') |\<in>| \<Gamma>,x:\<tau> \<longrightarrow> (y, \<tau>') |\<in>| \<Gamma>' \<Longrightarrow> \<Gamma>' \<turnstile>\<^sub>t\<^sub>y e : \<tau>\<^sub>2 ; \<forall>y\<in>FFVars_terms (Abs x \<tau> e). \<forall>\<tau>. (y, \<tau>) |\<in>| \<Gamma> \<longrightarrow> (y, \<tau>) |\<in>| \<Gamma>' \<rbrakk> \<Longrightarrow> \<Gamma>' \<turnstile>\<^sub>t\<^sub>y (Abs x \<tau> e) : (\<tau> \<rightarrow> \<tau>\<^sub>2)"
+shows "\<Gamma>' \<turnstile>\<^sub>t\<^sub>y e : \<tau>"
+  apply (rule mp[OF mp[OF spec[OF spec[OF
+          Ty_fresh_induct_param[of
+             "\<lambda>c. case c of (\<Gamma>, \<Gamma>', e) \<Rightarrow> \<Union>(Basic_BNFs.fsts ` fset \<Gamma>) \<union> \<Union>(Basic_BNFs.fsts ` fset \<Gamma>') \<union> FFVars_terms e" _ _ _
+             "\<lambda>\<Gamma> e \<tau> \<rho>. \<forall>\<Gamma>'. \<rho> = (\<Gamma>, \<Gamma>', e) \<longrightarrow> (\<forall>x\<in>FFVars_terms e. \<forall>\<tau>. (x, \<tau>) |\<in>| \<Gamma> \<longrightarrow> (x, \<tau>) |\<in>| \<Gamma>') \<longrightarrow> \<Gamma>' \<turnstile>\<^sub>t\<^sub>y e : \<tau>"
+      ]]] refl]])
+       apply (rule allI)
+  subgoal for \<rho>
+    apply (rule prod.exhaust[of \<rho>])
+    apply hypsubst_thin
+    subgoal for \<Gamma> p
+      apply (rule prod.exhaust[of p])
+      apply hypsubst_thin
+      unfolding prod.case
+      apply (rule terms_pre.Un_bound)+
+        apply (rule terms_pre.UNION_bound, rule ordLess_ordLeq_trans, raw_tactic \<open>resolve_tac @{context} (
+        BNF_Def.set_bd_of_bnf (the (BNF_Def.bnf_of @{context} "FSet.fset"))
+      ) 1\<close>, rule terms.var_large, rule ordLess_ordLeq_trans, raw_tactic \<open>resolve_tac @{context} (
+        BNF_Def.set_bd_of_bnf (the (BNF_Def.bnf_of @{context} @{type_name prod}))
+      ) 1\<close>, rule terms.var_large)+
+      apply (rule terms.set_bd_UNIV)
+      done
+    done
+      apply (rule assms(1))
+     apply (rule allI impI)+
+     apply (rule Var)
+      apply assumption+
+    apply (rule allI impI)+
+    apply (rule App)
+        apply assumption+
+      apply (erule allE)+
+      apply (erule impE)
+       apply (rule refl)
+      apply (rotate_tac -1)
+      apply (erule impE)
+       apply assumption
+      apply assumption
+     apply (erule allE)+
+     apply (rotate_tac -1)
+     apply (erule impE)
+      apply (rule refl)
+     apply (rotate_tac -1)
+     apply (erule impE)
+      apply assumption
+     apply assumption
+    apply assumption
+   apply (rule allI impI)+
+   apply (rule Abs)
+  apply (raw_tactic \<open>Subgoal.FOCUS_PARAMS (fn {context=ctxt, params, ...} =>
+    resolve_tac ctxt [infer_instantiate' ctxt [SOME (snd (nth params 5))] @{thm prod.exhaust}] 1
+  ) @{context} 1\<close>)
+    apply hypsubst_thin
+  unfolding prod.case
+       apply assumption+
+    apply (erule allE)+
+    apply (erule impE)
+     apply (rule refl)
+    apply (erule impE)
+     apply assumption+
+  apply (rule assms(2))
+  done
+(* TODO: automate with binder_induction method *)
+lemma substitution_induct:
+  assumes "\<Gamma>,x:\<tau>' \<turnstile>\<^sub>t\<^sub>y e : \<tau>" "x \<sharp> \<Gamma>" "{||} \<turnstile>\<^sub>t\<^sub>y v : \<tau>'"
+and Var: "\<And>a \<Gamma> \<tau>. \<lbrakk> \<Gamma>,x:\<tau>' \<turnstile>\<^sub>t\<^sub>y Var a : \<tau> ; x \<sharp> \<Gamma> ; {||} \<turnstile>\<^sub>t\<^sub>y v : \<tau>' \<rbrakk> \<Longrightarrow> \<Gamma> \<turnstile>\<^sub>t\<^sub>y tvsubst (VVr(x := v)) (Var a) : \<tau>"
+and App: "\<And>e1 e2 \<Gamma> \<tau>. \<lbrakk>
+    \<And>\<Gamma> \<tau>. \<Gamma>,x:\<tau>' \<turnstile>\<^sub>t\<^sub>y e1 : \<tau> \<Longrightarrow> x \<sharp> \<Gamma> \<Longrightarrow> {||} \<turnstile>\<^sub>t\<^sub>y v : \<tau>' \<Longrightarrow> \<Gamma> \<turnstile>\<^sub>t\<^sub>y tvsubst (VVr(x := v)) e1 : \<tau> ;
+    \<And>\<Gamma> \<tau>. \<Gamma>,x:\<tau>' \<turnstile>\<^sub>t\<^sub>y e2 : \<tau> \<Longrightarrow> x \<sharp> \<Gamma> \<Longrightarrow> {||} \<turnstile>\<^sub>t\<^sub>y v : \<tau>' \<Longrightarrow> \<Gamma> \<turnstile>\<^sub>t\<^sub>y tvsubst (VVr(x := v)) e2 : \<tau> ;
+    \<Gamma>,x:\<tau>' \<turnstile>\<^sub>t\<^sub>y App e1 e2 : \<tau> ; x \<sharp> \<Gamma> ; {||} \<turnstile>\<^sub>t\<^sub>y v : \<tau>'
+  \<rbrakk> \<Longrightarrow> \<Gamma> \<turnstile>\<^sub>t\<^sub>y tvsubst (VVr(x := v)) (App e1 e2) : \<tau>"
+and Abs: "\<And>y \<tau>\<^sub>1 e \<Gamma> \<tau>. \<lbrakk>
+    y \<notin> \<Union>(Basic_BNFs.fsts ` fset \<Gamma>) \<union> {x} \<union> FFVars_terms v ;
+    \<And>\<Gamma> \<tau>. \<Gamma>,x:\<tau>' \<turnstile>\<^sub>t\<^sub>y e : \<tau> \<Longrightarrow> x \<sharp> \<Gamma> \<Longrightarrow> {||} \<turnstile>\<^sub>t\<^sub>y v : \<tau>' \<Longrightarrow> \<Gamma> \<turnstile>\<^sub>t\<^sub>y tvsubst (VVr(x := v)) e : \<tau> ;
+    \<Gamma>,x:\<tau>' \<turnstile>\<^sub>t\<^sub>y Abs y \<tau>\<^sub>1 e : \<tau> ; x \<sharp> \<Gamma> ; {||} \<turnstile>\<^sub>t\<^sub>y v : \<tau>'
+  \<rbrakk> \<Longrightarrow> \<Gamma> \<turnstile>\<^sub>t\<^sub>y tvsubst (VVr(x := v)) (Abs y \<tau>\<^sub>1 e) : \<tau>"
+shows "\<Gamma> \<turnstile>\<^sub>t\<^sub>y tvsubst (VVr(x:=v)) e : \<tau>"
+apply (rule mp[OF spec[OF spec[OF spec[OF
+          TT_fresh_induct_param[of "\<lambda>\<rho>. \<Union>(Basic_BNFs.fsts ` fset \<rho>) \<union> {x} \<union> FFVars_terms v" "\<lambda>e \<rho>. \<forall>\<Gamma> \<tau>. (\<rho> = \<Gamma> \<and> \<Gamma>,x:\<tau>' \<turnstile>\<^sub>t\<^sub>y e : \<tau> \<and> x \<sharp> \<Gamma> \<longrightarrow> \<Gamma> \<turnstile>\<^sub>t\<^sub>y tvsubst (VVr(x:=v)) e : \<tau>)"]
+  ]]]])
+      apply (rule allI)
+      apply (rule terms_pre.Un_bound)+
+        apply (rule terms_pre.UNION_bound, rule ordLess_ordLeq_trans, raw_tactic \<open>resolve_tac @{context} (
+        BNF_Def.set_bd_of_bnf (the (BNF_Def.bnf_of @{context} "FSet.fset"))
+      ) 1\<close>, rule terms.var_large, rule ordLess_ordLeq_trans, raw_tactic \<open>resolve_tac @{context} (
+        BNF_Def.set_bd_of_bnf (the (BNF_Def.bnf_of @{context} @{type_name prod}))
+      ) 1\<close>, rule terms.var_large)+
+       apply (rule singl_bound)
+      apply (rule terms.set_bd_UNIV)
+     apply (rule allI impI)+
+     apply (erule conjE)+
+     apply (rule Var)
+       apply assumption+
+     apply (rule assms(3))
+    apply (rule allI impI)+
+    apply (erule conjE)+
+    apply (rule App)
+        apply (erule allE)+
+        apply (erule impE)
+         prefer 2
+         apply assumption
+        apply (rule conjI)
+         apply (rule refl)
+        apply (rule conjI)
+         apply assumption
+        apply assumption
+       apply (erule allE)+
+       apply (rotate_tac -1)
+       apply (erule impE)
+        prefer 2
+        apply assumption
+       apply (rule conjI)
+        apply (rule refl)
+       apply (rule conjI)
+        apply assumption+
+    apply (rule assms(3))
+   apply (rule allI impI)+
+   apply (erule conjE)+
+   apply (rule Abs)
+       apply hypsubst
+       apply assumption
+      apply (erule allE)+
+      apply (erule impE)
+       prefer 2
+       apply assumption
+      apply (rule conjI)
+  apply (rule refl)
+      apply (rule conjI)
+       apply assumption+
+   apply (rule assms(3))
+  apply (rule conjI)
+   apply (rule refl)
+  apply (rule conjI assms)+
+  done
 
 
 
-theorem progress: "[] \<turnstile>\<^sub>t\<^sub>y e : \<tau> \<Longrightarrow> (\<exists>x \<tau> e'. e = Abs x \<tau> e') \<or> (\<exists>e'. e \<longrightarrow> e')"
-proof (induction "[] :: ('a::var_terms_pre * \<tau>) list" e \<tau> rule: Ty.induct)
+
+
+
+
+lemma context_invariance: "\<Gamma> \<turnstile>\<^sub>t\<^sub>y e : \<tau>' \<Longrightarrow> \<forall>x\<in>FFVars_terms e. \<forall>\<tau>. (x, \<tau>) |\<in>| \<Gamma> \<longrightarrow> (x, \<tau>) |\<in>| \<Gamma>' \<Longrightarrow> \<Gamma>' \<turnstile>\<^sub>t\<^sub>y e : \<tau>'"
+proof (erule context_invariance_induct, assumption, goal_cases)
+  case (1 x \<tau> \<Gamma> \<Gamma>')
+  then show ?case by (auto intro: Ty_Var)
+next
+  case (2 \<Gamma> \<Gamma>' e1 \<tau>\<^sub>1 \<tau>\<^sub>2 e2)
+  then show ?case unfolding FFVars_terms_simps by (meson Ty_App UnI1 UnI2)
+next
+  case (3 x \<Gamma> \<Gamma>' \<tau> e \<tau>\<^sub>2)
+  then have "\<forall>y\<in>FFVars_terms e. \<forall>\<tau>'. (y, \<tau>') |\<in>| \<Gamma>,x:\<tau> \<longrightarrow> (y, \<tau>') |\<in>| \<Gamma>',x:\<tau>"
+    by (metis DiffI FFVars_terms_simps(3) fimageI finsert_iff fresh_def fst_conv fsts.cases prod_set_simps(1))
+  moreover have "x \<sharp> \<Gamma>'" using 3 unfolding fresh_def
+    by (metis UN_I UnI1 UnI2 fimageE fmember_iff_member_fset fsts.intros)
+  ultimately show ?case using 3 by (auto intro: Ty_Abs)
+qed
+
+lemma substitution: "\<lbrakk> \<Gamma>,x:\<tau>' \<turnstile>\<^sub>t\<^sub>y e : \<tau> ; x \<sharp> \<Gamma> ; {||} \<turnstile>\<^sub>t\<^sub>y v : \<tau>' \<rbrakk> \<Longrightarrow> \<Gamma> \<turnstile>\<^sub>t\<^sub>y tvsubst (VVr(x:=v)) e : \<tau>"
+proof (erule substitution_induct, assumption+, goal_cases)
+  case (1 a \<Gamma> \<tau>)
+  then have 2: "(a, \<tau>) |\<in>| \<Gamma>,x:\<tau>'" by blast
+  from \<open>{||} \<turnstile>\<^sub>t\<^sub>y v : \<tau>'\<close> have 3: "\<Gamma> \<turnstile>\<^sub>t\<^sub>y v : \<tau>'" using context_invariance by blast
+  then show ?case unfolding tvsubst_simps[OF SSupp_upd_VVr_bound] unfolding fun_upd_def
+  proof (cases "a = x")
+    case True
+    then have "\<tau> = \<tau>'" using 2 1(1) unfolding fresh_def
+      by (metis "1"(4) Pair_inject finsertE fresh_def fst_eqD rev_fimage_eqI)
+    then show "\<Gamma> \<turnstile>\<^sub>t\<^sub>y if a = x then v else VVr a : \<tau>" using True 3 by simp
+  next
+    case False
+    then have "(a, \<tau>) |\<in>| \<Gamma>" using 2 by blast
+    then show "\<Gamma> \<turnstile>\<^sub>t\<^sub>y if a = x then v else VVr a : \<tau>" unfolding VVr_eq_Var using False Ty.Ty_Var by auto
+  qed
+next
+  case (2 e1 e2 \<Gamma> \<tau>)
+  from 2(5) obtain \<tau>\<^sub>1 where "\<Gamma>,x:\<tau>' \<turnstile>\<^sub>t\<^sub>y e1 : \<tau>\<^sub>1 \<rightarrow> \<tau>" "\<Gamma>,x:\<tau>' \<turnstile>\<^sub>t\<^sub>y e2 : \<tau>\<^sub>1" by blast
+  then have "\<Gamma> \<turnstile>\<^sub>t\<^sub>y tvsubst (VVr(x := v)) e1 : \<tau>\<^sub>1 \<rightarrow> \<tau>" "\<Gamma> \<turnstile>\<^sub>t\<^sub>y tvsubst (VVr(x := v)) e2 : \<tau>\<^sub>1" using 2 by blast+
+  then have "\<Gamma> \<turnstile>\<^sub>t\<^sub>y App (tvsubst (VVr(x := v)) e1) (tvsubst (VVr(x := v)) e2) : \<tau>" using Ty_App by blast
+  then show ?case unfolding tvsubst_simps(2)[OF SSupp_upd_VVr_bound, symmetric] .
+next
+  case (3 y \<tau>\<^sub>1 e \<Gamma> \<tau>)
+  then have 1: "y \<notin> IImsupp (VVr(x:=v))" by (simp add: IImsupp_def SSupp_def)
+  have "y \<notin> \<Union>(Basic_BNFs.fsts ` fset (\<Gamma>,x:\<tau>'))" using 3(3) unfolding fresh_def by auto
+  then obtain \<tau>\<^sub>2 where 2: "(\<Gamma>,x:\<tau>'),y:\<tau>\<^sub>1 \<turnstile>\<^sub>t\<^sub>y e : \<tau>\<^sub>2" "\<tau> = (\<tau>\<^sub>1 \<rightarrow> \<tau>\<^sub>2)" using 3(5) Ty_AbsE' by metis
+  moreover have "(\<Gamma>,x:\<tau>'),y:\<tau>\<^sub>1 = (\<Gamma>,y:\<tau>\<^sub>1),x:\<tau>'" using 3(3) by blast
+  moreover have "x \<sharp> \<Gamma>,y:\<tau>\<^sub>1" using 3(3,6) unfolding fresh_def by auto
+  ultimately have "\<Gamma>,y:\<tau>\<^sub>1 \<turnstile>\<^sub>t\<^sub>y tvsubst (VVr(x := v)) e : \<tau>\<^sub>2" using 3(2,4) by auto
+  moreover have "y \<sharp> \<Gamma>" using 3(3) unfolding fresh_def
+    by (metis UN_I UnI1 fimageE fmember_iff_member_fset fsts.intros)
+  ultimately show ?case unfolding tvsubst_simps(3)[OF SSupp_upd_VVr_bound 1] using Ty_Abs 2(2) by blast
+qed
+
+
+
+
+theorem progress: "{||} \<turnstile>\<^sub>t\<^sub>y e : \<tau> \<Longrightarrow> (\<exists>x \<tau> e'. e = Abs x \<tau> e') \<or> (\<exists>e'. e \<longrightarrow> e')"
+proof (induction "{||} :: ('a::var_terms_pre * \<tau>) fset" e \<tau> rule: Ty.induct)
   case (Ty_App e1 \<tau>\<^sub>1 \<tau>\<^sub>2 e2)
   from Ty_App(2) show ?case using ST_Beta ST_App by blast
 qed auto
 
-lemma context_invariance: "\<lbrakk> \<Gamma> \<turnstile>\<^sub>t\<^sub>y e : \<tau> ; \<forall>x \<tau>'. (x, \<tau>') \<in> \<Gamma> \<longrightarrow> (x, \<tau>') \<in> \<Gamma>' \<rbrakk> \<Longrightarrow> \<Gamma>' \<turnstile>\<^sub>t\<^sub>y e : \<tau>"
-proof (induction \<Gamma> e \<tau> arbitrary: \<Gamma>' rule: Ty.induct)
-  case (Ty_Abs x \<Gamma> \<tau> e \<tau>\<^sub>2)
-  then have "\<forall>x' \<tau>'. (x', \<tau>') \<in> (x, \<tau>)#\<Gamma> \<longrightarrow> (x', \<tau>') \<in> (x, \<tau>)#\<Gamma>'" by auto
-  then show ?case using Ty_Abs Ty.Ty_Abs by blast
-qed (auto intro: Ty_Var Ty_App)
-
-lemma substitution: "\<lbrakk> (x, \<tau>')#\<Gamma> \<turnstile>\<^sub>t\<^sub>y e : \<tau> ; [] \<turnstile>\<^sub>t\<^sub>y v : \<tau>' \<rbrakk> \<Longrightarrow> \<Gamma> \<turnstile>\<^sub>t\<^sub>y tvsubst (VVr(x:=v)) e : \<tau>"
-proof (induction e arbitrary: \<Gamma> \<tau> rule: TT_fresh_induct[of "{x} \<union> FFVars_terms v"])
-  case Bound
-  then show ?case using terms_pre.Un_bound singl_bound terms.card_of_FFVars_bounds by fast
-next
-  case (Var a)
-  then have 2: "(a, \<tau>) \<in> (x, \<tau>') # \<Gamma>" by cases auto
-  have 3: "\<Gamma> \<turnstile>\<^sub>t\<^sub>y v : \<tau>'" using context_invariance[OF Var(2)] by simp
-  then show ?case unfolding tvsubst_simps[OF SSupp_upd_VVr_bound] unfolding fun_upd_def
-  proof (cases "a = x")
-    case True
-    then have "\<tau> = \<tau>'" using 2 by simp
-    then show "\<Gamma> \<turnstile>\<^sub>t\<^sub>y if a = x then v else VVr a : \<tau>" using True 3 by simp
-  next
-    case False
-    then have 4: "(a, \<tau>) \<in> \<Gamma>" using 2 by simp
-    show "\<Gamma> \<turnstile>\<^sub>t\<^sub>y if a = x then v else VVr a : \<tau>" unfolding VVr_eq_Var using False Ty.Ty_Var[OF 4] by simp
-  qed
-next
-  case (App e1 e2)
-  from App(3) obtain \<tau>1 where "(x, \<tau>') # \<Gamma> \<turnstile>\<^sub>t\<^sub>y e1 : \<tau>1 \<rightarrow> \<tau>" "(x, \<tau>') # \<Gamma> \<turnstile>\<^sub>t\<^sub>y e2 : \<tau>1" by cases auto
-  then have "\<Gamma> \<turnstile>\<^sub>t\<^sub>y tvsubst (VVr(x := v)) e1 : \<tau>1 \<rightarrow> \<tau>" "\<Gamma> \<turnstile>\<^sub>t\<^sub>y tvsubst (VVr(x := v)) e2 : \<tau>1" using App by blast+
-  then have "\<Gamma> \<turnstile>\<^sub>t\<^sub>y App (tvsubst (VVr(x := v)) e1) (tvsubst (VVr(x := v)) e2) : \<tau>" using Ty_App by blast
-  then show ?case unfolding tvsubst_simps(2)[OF SSupp_upd_VVr_bound, symmetric] .
-next
-  case (Abs y \<tau>1 e)
-  then have 1: "y \<notin> IImsupp (VVr(x:=v))" by (simp add: IImsupp_def SSupp_def)
-  from Abs(3) have "\<exists>y' e' \<tau>2. (y', \<tau>1)#(x, \<tau>')#\<Gamma> \<turnstile>\<^sub>t\<^sub>y e' : \<tau>2 \<and> Abs y \<tau>' e = Abs y' \<tau>' e' \<and> y' \<noteq> x \<and> \<tau> = (\<tau>1 \<rightarrow> \<tau>2)"
-  proof cases
-    case (Ty_Abs y' \<tau>1' e' \<tau>\<^sub>2)
-    then obtain y'' e'' where "Abs y \<tau>1 e = Abs y'' \<tau>1 e''" "y'' \<noteq> x" using Abs_avoid[OF singl_bound[of x]] by blast
-    then show ?thesis using Ty_Abs sorry
-  qed auto
-  
-  show ?case unfolding tvsubst_simps(3)[OF SSupp_upd_VVr_bound 1] using Abs sorry
-qed
-
-theorem preservation: "\<lbrakk> [] \<turnstile>\<^sub>t\<^sub>y e : \<tau> ; e \<longrightarrow> e' \<rbrakk> \<Longrightarrow> [] \<turnstile>\<^sub>t\<^sub>y e' : \<tau>"
-proof (induction "[] :: ('a::var_terms_pre * \<tau>) list" e \<tau> arbitrary: e' rule: Ty.induct)
+theorem preservation: "\<lbrakk> {||} \<turnstile>\<^sub>t\<^sub>y e : \<tau> ; e \<longrightarrow> e' \<rbrakk> \<Longrightarrow> {||} \<turnstile>\<^sub>t\<^sub>y e' : \<tau>"
+proof (induction "{||} :: ('a::var_terms_pre * \<tau>) fset" e \<tau> arbitrary: e' rule: Ty.induct)
   case (Ty_App e1 \<tau>\<^sub>1 \<tau>\<^sub>2 e2)
   from Ty_App(5) show ?case
   proof cases
     case (ST_Beta x \<tau> e e2')
-    then have "[] \<turnstile>\<^sub>t\<^sub>y App (Abs x \<tau> e) e2 : \<tau>\<^sub>2" using Ty_App Ty.Ty_App by fastforce
-    then have "[] \<turnstile>\<^sub>t\<^sub>y tvsubst (VVr(x := e2)) e : \<tau>\<^sub>2" using Ty_App sorry
+    then have "{||} \<turnstile>\<^sub>t\<^sub>y App (Abs x \<tau> e) e2 : \<tau>\<^sub>2" using Ty_App Ty.Ty_App by fastforce
+    have "{||} \<turnstile>\<^sub>t\<^sub>y Abs x \<tau>\<^sub>1 e : \<tau>\<^sub>1 \<rightarrow> \<tau>\<^sub>2" using Ty_App ST_Beta
+      by (smt (verit, ccfv_SIG) Abs_inject App_inject Ty.cases \<tau>.inject terms_distinct(2) terms_distinct(4))
+    then have "{||},x:\<tau>\<^sub>1 \<turnstile>\<^sub>t\<^sub>y e : \<tau>\<^sub>2" by (auto elim: Ty_AbsE')
+    then have "{||} \<turnstile>\<^sub>t\<^sub>y tvsubst (VVr(x := e2')) e : \<tau>\<^sub>2" using substitution ST_Beta(1) Ty_App(3) unfolding fresh_def by fastforce
     then show ?thesis using ST_Beta by simp
   next
     case (ST_App e e1' e2')
-    then have "[] \<turnstile>\<^sub>t\<^sub>y e1' : \<tau>\<^sub>1 \<rightarrow> \<tau>\<^sub>2" using Ty_App by simp
+    then have "{||} \<turnstile>\<^sub>t\<^sub>y e1' : \<tau>\<^sub>1 \<rightarrow> \<tau>\<^sub>2" using Ty_App by simp
     then show ?thesis using Ty_App Ty.Ty_App ST_App by fastforce
   qed
 next
   case (Ty_Abs x \<tau> e \<tau>\<^sub>2)
-  from Ty_Abs(2) show ?case by cases auto
+  from \<open>Abs x \<tau> e \<longrightarrow> e'\<close> show ?case by cases auto
 qed auto
 
 end
